theories/regex.v
@@ -1,65 +1,76 @@
-(* Definition of regular expression on alphabet T 
+Require Import Coq.Strings.Ascii.
+Require Import Coq.Strings.String.
+(* Require Import Coq.Sets.Ensembles. *)
+From SetsClass Require Import SetsClass.
+Local Open Scope sets_scope.
+Local Open Scope list_scope.
+(* Definition of regular expressiontheories/st_graph_nfa.v theories/st_nograph_nfa.v on alphabet T 
    in Software Foundations *)
-(* TODO: add '()' '[]' '{n}' *)
+(*? remove Question/Plus *)
 
-Inductive reg_exp (T : Type) : Type :=
+(* TODO: Denotational defined regex *)
+(* String -> Prop *)
+(* Star r := Union (r^0, r^1, ..., r^n)  *)
+(* CS2612 *)
+
+Inductive reg_exp (T: Type) : Type :=
   (* Ø *)
-  | EmptySet
+  | EmptySet_r
   (* '' *)
-  | EmptyStr
+  | EmptyStr_r
   (* 't' *)
-  | Char (t : T)
+  | Char_r (t : T)
   (* '<r1><r2>' *)
-  | Concat (r1 r2 : reg_exp T)
+  | Concat_r (r1 r2 : reg_exp T)
   (* '<r1>|<r2>' *)
-  | Union (r1 r2 : reg_exp T)
+  | Union_r (r1 r2 : reg_exp T)
   (* '<r>*' *)
-  | Star (r : reg_exp T)
-  (* '<r>?' *)
-  | Question (r : reg_exp T)
-  (* '<r>+' *)
-  | Plus (r : reg_exp T).
+  | Star_r (r : reg_exp T).
 
-Arguments EmptySet {T}.
-Arguments EmptyStr {T}.
-Arguments Char {T} _.
-Arguments Concat {T} _ _.
-Arguments Union {T} _ _.
-Arguments Star {T} _.
-Arguments Question {T} _.
-Arguments Plus {T} _.
+Arguments EmptySet_r {T}.
+Arguments EmptyStr_r {T}.
+Arguments Char_r {T} _.
+Arguments Concat_r {T} _ _.
+Arguments Union_r {T} _ _.
+Arguments Star_r {T} _.
 
-Reserved Notation "s =~ re" (at level 80).
+(* Inductive Concat_Ensemble (B C : Ensemble string) : Ensemble string :=
+  Concat_intro : forall (x y : string), In string B x -> In string C y -> In string (Concat_Ensemble B C) (x ++ y). *)
 
 (* If the string can be matched by the reg_exp *)
-Inductive exp_match {T} : list T -> reg_exp T -> Prop :=
-  | MEmpty : nil =~ EmptyStr
-  | MChar x : cons x nil =~ (Char x)
-  | MConcat s1 re1 s2 re2
-             (H1 : s1 =~ re1)
-             (H2 : s2 =~ re2)
-           : (s1 ++ s2) =~ (Concat re1 re2)
-  | MUnionL s1 re1 re2
-                (H1 : s1 =~ re1)
-              : s1 =~ (Union re1 re2)
-  | MUnionR re1 s2 re2
-                (H2 : s2 =~ re2)
-              : s2 =~ (Union re1 re2)
-  | MStar0 re : nil =~ (Star re)
-  | MStarApp s1 s2 re
-                 (H1 : s1 =~ re)
-                 (H2 : s2 =~ (Star re))
-               : (s1 ++ s2) =~ (Star re)
-  | MQuestion0 re : nil =~ (Question re)
-  | MQuestion1 s re
-               (H : s =~ re)
-               : s =~ (Question re)
-  | MPlus1 s re
-            (H : s =~ re)
-            : s =~ (Plus re)
-  | MPlusApp s1 s2 re
-                 (H1 : s1 =~ re)
-                 (H2 : s2 =~ (Plus re))
-               : (s1 ++ s2) =~ (Plus re)
+  (* set string *)
 
-  where "s =~ re" := (exp_match s re).
+Check Sets.full .
+Check Sets.equiv .
+
+Check forall A (X: A -> Prop), X ∪ ∅ == X.
+Check forall A B (X Y: A -> B -> Prop), X ∪ Y ⊆ X.
+
+Definition set_prod {T} (A B : list T -> Prop) : list T -> Prop :=
+  fun s => exists s1 s2, s1 ∈ A /\ s2 ∈ B /\ s = s1 ++ s2.
+
+Print Sets.indexed_union .
+
+Fixpoint star_r_indexed {T} (n : nat) (s : list T -> Prop) : list T -> Prop :=
+  match n with
+  | 0 => [ nil ]
+  | S n' => set_prod s (star_r_indexed n' s)
+  end.
+
+Fixpoint exp_match {T} (r : reg_exp T) : list T -> Prop :=
+  match r with
+  | EmptySet_r => ∅
+  | EmptyStr_r => [ nil ]
+  | Char_r t => [ (cons t nil) ]
+  | Concat_r r1 r2 => set_prod (exp_match r1) (exp_match r2)
+  | Union_r r1 r2 => (exp_match r1) ∪ (exp_match r2)
+  | Star_r r => ⋃ star_r_indexed (exp_match r)
+  end.
+
+(** Proof: exp_match *)
+(** (v_n,v_m) <= (v_n', v_m') *)
+(** interval (v_n,v_m) return_graph (v_n', v_m') *)
+(** correctness *)
+(** 1. st_graph: Hoare triple definition + Admitted. *)
+(** 2. Refinement proof between st_nograph and st_graph *)
+(** forall G: graph, (low_level state = G & alloc same val), execute, (ret val start,end same , Hi ret graph ⋃ G = G') *)
