theories/hoare.v
@@ -1,0 +1,60 @@
+Require Import Regex2NFA.lib.PreGraph.
+Require Import Regex2NFA.theories.st_graph_nfa.
+Require Import Regex2NFA.theories.st_nograph_nfa.
+Require Import Regex2NFA.theories.regex.
+Require Import Coq.ZArith.ZArith.
+From StateMonad.monaderror Require Import monadEbasic.
+From StateMonad.monaderror Require Import monadEhoare.
+
+Import MonadNotation.
+Local Open Scope stmonad_scope.
+Local Open Scope Z_scope.
+
+(** high_level prop *)
+Lemma st_nograph_inc {T: Type} :
+  forall (G: @pg_nfa T) (r: reg_exp T), exists (v e : Z),
+  Hoare (fun s1 => s1.(max_v) = v /\
+                   s1.(max_e) = e)
+        (regexToNFA r)
+        (fun el s2 => el.(startVertex) >= v /\
+                      el.(endVertex) >= v /\
+                      G_disjoint G el.(graph) ).
+Proof.
+Admitted.
+
+(** high_level (st_nograph)
+(v, e)
+(sv, ev, G_ret) <- execute
+(v', e')
+*)
+(** low_level (st_graph)
+(v, e, G)
+(sv, ev) <- execute'
+(v', e', G')
+*)
+(* Lemma graph_corr_prop {T: Type} :
+  forall (G: @pg_nfa T) (r: reg_exp T) (v e: Z),
+  exists (G_ret: @pg_nfa T) (v' e' sv ev : Z),
+  (** low_level : @Hoare state' elem' *)
+  Hoare (fun s1 => s1.(st_graph) = G /\
+                   s1.(max_v') = v /\
+                   s1.(max_e') = e )
+        (regexToNFA' r)
+        (fun el s2 => s2.(max_v') = v' /\
+                      s2.(max_e') = e' /\
+                      G1_union G G_ret s2.(st_graph) ) /\
+  (** high_level : @Hoare state elem *)
+  Hoare (fun s1 => s1.(max_v) = v /\
+                   s1.(max_e) = e)
+        (regexToNFA r)
+        (fun el s2 => s2.(max_v) = v' /\
+                      s2.(max_e) = e' /\
+                      el.(startVertex) = sv /\
+                      el.(endVertex) = ev /\
+                      el.(graph) = G_ret).
+  (* v' >= v /\ e' >= e *)
+  (* sv > v /\ sv <= v' /\ ev > v /\ ev <= v' *)
+  (** el.(graph) rel *)
+  (*? edge rel *)
+Proof.
+Admitted. *)
